FSharpNemlogIn/FStarWrapper/CryptoTest.fs
@@ -4,21 +4,21 @@ open System.Security.Cryptography
 open Network
 open Crypto
 
-let TestCrypto = 
-    let spid = "https://saml.serviceprovicer.org"
-    let idpid = "https://saml.identityprovicer.org"
-    let (privk, pubk) = KeyGenExt spid
-    
-    let msg = X.GetReq spid idpid
-    printfn "Message to sign %s" msg
-
-    let signature = SignMessage spid privk msg
-    printfn "Message signature: %s" signature
-    
-    printfn "Verifying signature"
-    let isValid = ValidateMessage "me" pubk msg signature
-    if isValid then
-        printfn "Signature: %s is valid" signature
-    else
-        printfn "Invalid Signature: %s" signature
+//let TestCrypto = 
+//    let spid = "https://saml.serviceprovicer.org"
+//    let idpid = "https://saml.identityprovicer.org"
+//    let (privk, pubk) = KeyGenExt spid
+//    
+//    let msg = X.GetReq spid idpid
+//    printfn "Message to sign %s" msg
+//
+//    let signature = SignMessage spid privk.y_0_342 msg
+//    printfn "Message signature: %s" signature
+//    
+//    printfn "Verifying signature"
+//    let isValid = ValidateMessage "me" pubk.y_0_343 msg signature
+//    if isValid then
+//        printfn "Signature: %s is valid" signature
+//    else
+//        printfn "Invalid Signature: %s" signature
 
