FSharpNemlogIn/FStarWrapper/Program.fs
@@ -3,16 +3,17 @@ open System.Security.Cryptography
 open Network
 open CryptoTest
 
+let rec StartListen() =
+    xServer.server "sp" "idp"
+    let key = Console.ReadKey ()
+    match key.KeyChar with
+    | 'x' -> ()
+    | _ -> StartListen()
+
+
 [<EntryPoint>]
 let main argv = 
-    
-//    let keys = Protocol.KeyGenExt "me"
-//    let priv = keys.__tag
-    
-    //let _ = TestCrypto  
-    let req = X.GetSamlMessages "sp" "idp"
-            
-    let _ = X.CreateSendAndRecieve "sp" "idp"
-   
-    let key = Console.Read ()
-    0 // return an integer exit code
+  
+  let x = X.GenKeys("some important principal")
+  let key = Console.Read ()
+  0 // return an integer exit code
