FSharpNemlogIn/WebServer/WebServerWebAppApi/ServiceProviderController.fs
@@ -1,2 +1,11 @@
-﻿module ServiceProviderController
+﻿namespace FsWeb.Controllers
 
+open System.Web
+open System.Web.Mvc
+open System.Net.Http
+open System.Web.Http
+
+type ServiceProviderController() =
+    inherit ApiController()
+
+    member x.Get() = ()
