Protocol/xserver.fst
@@ -1,0 +1,17 @@
+module xServer
+
+open Protocol
+open FstNetwork
+
+val server: string -> string -> unit
+let server sp idp = 
+  let msg = RecieveX "sp" in
+  match msg with
+  | HttpGet (uri) -> 
+    let authReq = CreateAuthnRequest sp idp in
+    let req = SamlProtocolMessage sp authReq "sig" in
+    let status = SendX "sp" req in
+    match status with
+    | true -> print_string "great!";()
+    | false -> print_string "crap!";()
+  | _ -> print_string "Oh shit!";()
